disj/DisjPaths.v
@@ -3,7 +3,7 @@ Require Export DisjDef MaxPreSuffix.
 Section disj.
   Context `{C : redCFG}.
   
-  Infix "⊴" := tagle (at level 70).
+  Infix "⊴" := Tagle (at level 70).
   
   Notation "p '-a>b' q" := (a_edge p q) (at level 55).
   Notation "p '-a>' q" := (p -a>b q = true) (at level 55).
